nola/examples/logic.v
@@ -119,13 +119,13 @@ Section iris.
     iSplit; (iIntros "[%[$[ihd itl]]]"; iSplitL "ihd";
       [iRevert "ihd"|iRevert "itl"]);
       iApply inv'_acsr; iIntros "!>" (??[eqv ?]).
+    - iApply bi.and_elim_l. iApply "eqv"; [|done]. iPureIntro.
+      by apply Deriv_mono=> ?[??].
+    - iApply (wand_iff_acsr (M:=fupd _ _)). iModIntro. by iApply eqv.
     - iApply bi.and_elim_r. iApply "eqv"; [|done]. iPureIntro.
       by apply Deriv_mono=> ?[??].
     - iApply (wand_iff_acsr (M:=fupd _ _)). iModIntro. rewrite wand_iff_comm.
       by iApply eqv.
-    - iApply bi.and_elim_l. iApply "eqv"; [|done]. iPureIntro.
-      by apply Deriv_mono=> ?[??].
-    - iApply (wand_iff_acsr (M:=fupd _ _)). iModIntro. by iApply eqv.
   Qed.
   Lemma ilist_acsr `{!Deriv ih δ} {N Φx Ψx l} :
     □ (∀ δ' l', ⌜Deriv ih δ'⌝ → ⌜ih δ'⌝ →
@@ -136,11 +136,11 @@ Section iris.
     iIntros "#eqv". rewrite /⟦ ⟧(δ) /=.
     iSplit; (iIntros "[ihd itl]"; iSplitL "ihd"; [iRevert "ihd"|iRevert "itl"]);
       iApply inv'_acsr; iIntros "!>" (???).
+    - iApply bi.and_elim_l. by iApply "eqv".
+    - iApply (wand_iff_acsr (M:=fupd _ _)). iModIntro. by iApply ilist'_acsr.
     - iApply bi.and_elim_r. by iApply "eqv".
     - iApply (wand_iff_acsr (M:=fupd _ _)). iModIntro. rewrite wand_iff_comm.
       by iApply ilist'_acsr.
-    - iApply bi.and_elim_l. by iApply "eqv".
-    - iApply (wand_iff_acsr (M:=fupd _ _)). iModIntro. by iApply ilist'_acsr.
   Qed.
 
   (** ** Termination of [iter] *)
